more

Weidenbach_Book/Watched_Literals/Watched_Literals_Algorithm_Restart.thy
@@ -1,5 +1,6 @@
 theory Watched_Literals_Algorithm_Restart
 imports Watched_Literals_Algorithm Watched_Literals_Transition_System_Restart
+  Weidenbach_Book_Base.Explorer
 begin
 
 context twl_restart_ops
@@ -13,45 +14,61 @@ text \<open>
   not manage to write the proof.
 \<close>
 text \<open>Restarts are never necessary\<close>
+definition GC_required :: "'v twl_st \<Rightarrow> nat \<Rightarrow> nat \<Rightarrow> bool nres" where
+  \<open>GC_required S last_GC_learnt_clss n = SPEC (\<lambda>b. b \<longrightarrow> size (get_all_learned_clss S) - last_GC_learnt_clss > f n)\<close>
 definition restart_required :: "'v twl_st \<Rightarrow> nat \<Rightarrow> nat \<Rightarrow> bool nres" where
-  \<open>restart_required S m n = SPEC (\<lambda>b. b \<longrightarrow> size (get_all_learned_clss S) - m > f n)\<close>
+  \<open>restart_required S last_Restart_learnt_clss n = SPEC (\<lambda>b. b \<longrightarrow> size (get_all_learned_clss S) > last_Restart_learnt_clss)\<close>
 
 definition (in -) restart_prog_pre :: \<open>'v twl_st \<Rightarrow> bool \<Rightarrow> bool\<close> where
   \<open>restart_prog_pre S brk \<longleftrightarrow> twl_struct_invs S \<and> twl_stgy_invs S \<and>
     (\<not>brk \<longrightarrow> get_conflict S = None)\<close>
 
 definition restart_prog
-  :: \<open>'v twl_st \<Rightarrow> nat \<Rightarrow> nat \<Rightarrow> bool \<Rightarrow> (bool \<times> 'v twl_st \<times> nat \<times> nat) nres\<close>
+  :: \<open>'v twl_st \<Rightarrow> 'v twl_st \<Rightarrow> 'v twl_st \<Rightarrow> nat \<Rightarrow> nat \<Rightarrow> bool \<Rightarrow> ('v twl_st \<times> 'v twl_st \<times> 'v twl_st \<times> nat \<times> nat) nres\<close>
 where
-  \<open>restart_prog S m n brk = do {
+  \<open>restart_prog last_GC last_Restart S m n brk = do {
      ASSERT(restart_prog_pre S brk);
-     b \<leftarrow> restart_required S m n;
-     b2 \<leftarrow> SPEC(\<lambda>_. b \<longrightarrow> size (get_all_learned_clss S) > m);
-     if b2 \<and> b \<and> \<not>brk then do {
+     b \<leftarrow> GC_required S (size (get_all_learned_clss last_GC))  n;
+     b2 \<leftarrow> restart_required S  (size (get_all_learned_clss last_Restart))  n;
+     if b2 \<and> \<not>brk then do {
        T \<leftarrow> SPEC(\<lambda>T. cdcl_twl_restart_only S T);
-       RETURN (True, T, size (get_all_learned_clss T), n)
+       RETURN (last_GC, T, T, Suc m, n)
      }
      else
      if b \<and> \<not>brk then do {
        T \<leftarrow> SPEC(\<lambda>T. cdcl_twl_restart S T);
        U \<leftarrow> SPEC(\<lambda>U. cdcl_twl_stgy\<^sup>*\<^sup>* T U \<and> clauses_to_update U = {#} \<and>
           get_conflict U = None);
-       RETURN (True, U, size (get_all_learned_clss U), n + 1)
+       RETURN (U, U, U, m, Suc n)
      }
      else
-       RETURN (False, S, m, n)
+       RETURN (last_GC, last_Restart, S, m, n)
    }\<close>
 
 fun cdcl_twl_stgy_restart_prog_inv where
-  \<open>cdcl_twl_stgy_restart_prog_inv S\<^sub>0 (brk, S, T, m, n) \<longleftrightarrow>
-    twl_struct_invs S\<^sub>0 \<and>
-    twl_struct_invs T \<and> twl_stgy_invs T \<and>
+  \<open>cdcl_twl_stgy_restart_prog_inv S\<^sub>0 (brk, R, S, T, m, n) \<longleftrightarrow>
+    twl_restart_inv (S\<^sub>0, S\<^sub>0, S\<^sub>0, 0, 0, True) \<and>
+    twl_stgy_restart_inv (S\<^sub>0, S\<^sub>0, S\<^sub>0, 0, 0, True) \<and>
     (brk \<longrightarrow> final_twl_state T) \<and>
-    cdcl_twl_stgy_restart_with_leftovers (S\<^sub>0, 0, True) m S (T, n, True) \<and>
+    cdcl_twl_stgy_restart\<^sup>*\<^sup>* (S\<^sub>0, S\<^sub>0, S\<^sub>0, 0, 0, True) (R, S, T, m, n, \<not>brk) \<and>
     clauses_to_update T = {#} \<and> (\<not>brk \<longrightarrow> get_conflict T = None)\<close>
 
 lemmas cdcl_twl_stgy_restart_prog_inv_def[simp del] =
   cdcl_twl_stgy_restart_prog_inv.simps
+
+lemma cdcl_twl_stgy_restart_prog_inv_alt_def:
+  \<open>cdcl_twl_stgy_restart_prog_inv S\<^sub>0 (brk, R, S, T, m, n) \<longleftrightarrow>
+    twl_restart_inv (S\<^sub>0, S\<^sub>0, S\<^sub>0, 0, 0, True) \<and>
+    twl_stgy_restart_inv (S\<^sub>0, S\<^sub>0, S\<^sub>0, 0, 0, True) \<and>
+    twl_stgy_restart_inv (R, S, T, m, n, \<not>brk) \<and>
+    twl_restart_inv (R, S, T, m, n, \<not>brk) \<and>
+    (brk \<longrightarrow> final_twl_state T) \<and>
+    cdcl_twl_stgy_restart\<^sup>*\<^sup>* (S\<^sub>0, S\<^sub>0, S\<^sub>0, 0, 0, True) (R, S, T, m, n, \<not>brk) \<and>
+  clauses_to_update T = {#} \<and> (\<not>brk \<longrightarrow> get_conflict T = None)\<close>
+  unfolding cdcl_twl_stgy_restart_prog_inv_def
+  by (auto dest: rtranclp_cdcl_twl_stgy_restart_twl_restart_inv
+    rtranclp_cdcl_twl_stgy_restart_twl_stgy_restart_inv)
+
 
 text \<open>
   In the main loop, and purely to simplify the proof, we remember the state obtained after the last
@@ -64,290 +81,84 @@ text \<open>
 definition cdcl_twl_stgy_restart_prog :: "'v twl_st \<Rightarrow> 'v twl_st nres" where
   \<open>cdcl_twl_stgy_restart_prog S\<^sub>0 =
   do {
-    (brk, _, T, _, _) \<leftarrow> WHILE\<^sub>T\<^bsup>cdcl_twl_stgy_restart_prog_inv S\<^sub>0\<^esup>
+    (brk, _, _, T, _, _) \<leftarrow> WHILE\<^sub>T\<^bsup>cdcl_twl_stgy_restart_prog_inv S\<^sub>0\<^esup>
       (\<lambda>(brk, _). \<not>brk)
-      (\<lambda>(brk, S, S', m, n).
+      (\<lambda>(brk, S, S', S'', m,  n).
       do {
         T \<leftarrow> unit_propagation_outer_loop S';
         (brk, T) \<leftarrow> cdcl_twl_o_prog T;
-        (b, T, m', n') \<leftarrow> restart_prog T m n brk;
-        RETURN (brk, if b then T else S, T, m', n')
+        (S, S', T, m', n') \<leftarrow> restart_prog S S' T m n brk;
+        RETURN (brk, S, S', T, m', n')
       })
-      (False, S\<^sub>0, S\<^sub>0, size (get_all_learned_clss S\<^sub>0), 0);
+      (False, S\<^sub>0, S\<^sub>0, S\<^sub>0, 0, 0);
     RETURN T
   }\<close>
 
-abbreviation cdcl_algo_termination_rel :: \<open>((bool \<times> 'v twl_st \<times> 'v twl_st \<times> nat \<times> nat) \<times> _) set\<close> where
-  \<open>cdcl_algo_termination_rel \<equiv>
-    {((brkT, T, T', n, n'), brkS, S, _, m, m').
-                              twl_struct_invs S \<and>
-                              \<not> brkS \<and>
-                              cdcl_twl_stgy_restart_with_leftovers1
-                             (S, m', \<not>brkS) (T, n', \<not>brkT)} \<union>
-                           {((brkT, T, T', n, n'), (brkS, S, S', m, m')). S = T \<and> \<not> brkS \<and> n' = m' \<and>
-                             twl_struct_invs S' \<and> cdcl_twl_stgy\<^sup>+\<^sup>+ S' T'} \<union>
-                           {((brkT, T), brkS, S). S = T \<and> brkT \<and> \<not> brkS}\<close>
+(* abbreviation cdcl_algo_termination_rel :: \<open>((bool \<times> 'v twl_st \<times> nat \<times> nat\<times> nat) \<times> _) set\<close> where
+ *   \<open>cdcl_algo_termination_rel \<equiv>
+ *     {((brkT, T, lgc', lrc', n'), brkS, S, lgc, lrc, n).
+ *                               \<not> brkS \<and>
+ *        (\<exists>Q Q' R R' m m'. twl_restart_inv (Q, R, S, m, n, \<not>brkS) \<and>
+ *          cdcl_twl_stgy_restart (Q, R, S, m, n, \<not>brkS) (Q', R', T, m', n', \<not>brkT))} \<union>
+ *    {((brkT, T), brkS, S). S = T \<and> brkT \<and> \<not> brkS}\<close> *)
 
 abbreviation cdcl_algo_termination_early_rel
-  :: \<open>((bool \<times> bool \<times> 'v twl_st \<times> 'v twl_st \<times> nat \<times> nat) \<times> _) set\<close>
+  :: \<open>((bool \<times> bool \<times> 'v twl_st \<times> 'v twl_st \<times>  'v twl_st \<times> nat \<times> nat) \<times> _) set\<close>
 where
   \<open>cdcl_algo_termination_early_rel \<equiv>
-    {((ebrkT, brkT, T, T', n, n'), ebrkS, brkS, S, _, m, m').
-                              twl_struct_invs S \<and>
-                              \<not> brkS \<and>
-                              cdcl_twl_stgy_restart_with_leftovers1
-                             (S, m', \<not>brkS) (T, n', \<not>brkT)} \<union>
-    {((ebrkT, brkT, T, T', n, n'), (ebrkS, brkS, S, S', m, m')). S = T \<and> \<not> brkS\<and> \<not> ebrkS \<and> n' = m' \<and>
-                             twl_struct_invs S' \<and> cdcl_twl_stgy\<^sup>+\<^sup>+ S' T'} \<union>
-    {((ebrkT, brkT, T), ebrkS, brkS, S). S = T \<and> (ebrkT \<or> brkT) \<and> \<not> brkS \<and> brkT}\<close>
+  {((ebrkT :: bool, brkT :: bool, R' :: 'v twl_st, S' :: 'v twl_st, T' :: 'v twl_st, m' :: nat, n' :: nat),
+       (ebrkS, brkS, R :: 'v twl_st, S :: 'v twl_st, T :: 'v twl_st, m :: nat, n :: nat)).
+     twl_restart_inv (R, S, T, m, n, \<not>brkS) \<and> \<not>brkS \<and>
+     cdcl_twl_stgy_restart\<^sup>+\<^sup>+ (R, S, T, m, n, \<not>brkS) (R', S', T', m', n', \<not>brkT)} \<union>
+  {((ebrkT :: bool, brkT :: bool, R' :: 'v twl_st, S' :: 'v twl_st, T' :: 'v twl_st, m' :: nat, n' :: nat),
+  (ebrkS, brkS, R :: 'v twl_st, S :: 'v twl_st, T :: 'v twl_st, m :: nat, n :: nat)).
+  \<not>brkS \<and> brkT}\<close>
+
 end
 
 
 context twl_restart
 begin
 
-lemma  wf_cdcl_algo_termination_early_rel: \<open>wf cdcl_algo_termination_early_rel\<close>
-  apply (rule wf_union_compatible)
-  apply (rule wf_union_compatible)
-  subgoal
-    by (rule wf_if_measure_in_wf[OF wf_cdcl_twl_stgy_restart_with_leftovers1,
-        of _  \<open>\<lambda>(_, brkT, T, T', n, n'). (T, n', \<not>brkT)\<close>])
-      auto
-  subgoal
-    by (rule wf_if_measure_in_wf[OF tranclp_wf_cdcl_twl_stgy,
-        of _  \<open>\<lambda>(_, brkT, T, T', n, n'). T'\<close>])
-      auto
-  subgoal
-    by auto
-  subgoal
-    by (rule wf_no_loop) auto
-  subgoal
-    by auto
-  done
+lemma cdcl_twl_stgy_restart_tranclpI:
+  \<open>cdcl_twl_stgy\<^sup>+\<^sup>+ T U \<Longrightarrow> cdcl_twl_stgy_restart\<^sup>+\<^sup>+ (R, S, T, m, n, True) (R, S, U, m, n, True)\<close>
+  by (induction rule: tranclp_induct)
+    (auto dest!: cdcl_twl_stgy_restart.intros(1)[of _ _ R S m n])
 
-lemma  wf_cdcl_algo_termination_rel: \<open>wf cdcl_algo_termination_rel\<close>
-  by (rule wf_if_measure_in_wf[OF wf_cdcl_algo_termination_early_rel,
-      of _  \<open>\<lambda>(brkT, T, T', n, n'). (False, brkT, T, T', n, n')\<close>])
-    auto
+lemma cdcl_twl_stgy_restart_rtranclpI:
+  \<open>cdcl_twl_stgy\<^sup>*\<^sup>* T U \<Longrightarrow> cdcl_twl_stgy_restart\<^sup>*\<^sup>* (R, S, T, m, n, True) (R, S, U, m, n, True)\<close>
+  by (induction rule: rtranclp_induct)
+    (auto dest!: cdcl_twl_stgy_restart.intros(1)[of _ _ R S m n])
 
-lemma restart_prog_spec:
-  assumes
-    inv: \<open>(cdcl_twl_stgy_restart_prog_inv S o snd) (ebrkU, brkU, T, U, m, n)\<close> and
-    cond: \<open>case (ebrkU, brkU, T, U, m, n) of (ebrk, brk, uu_) \<Rightarrow> \<not> brk \<and> \<not>ebrk\<close> and
-    other_inv: \<open>cdcl_twl_o_prog_spec V (brkT, W)\<close> and
-    struct_invs_V: \<open>twl_struct_invs V\<close> and
-    cp: \<open>cdcl_twl_cp\<^sup>*\<^sup>* U V\<close> and
-    lits_to_update: \<open>literals_to_update V = {#}\<close> and
-    \<open>\<forall>S'. \<not> cdcl_twl_cp V S'\<close> and
-    \<open>twl_stgy_invs V\<close>
-  shows \<open>restart_prog W m n brkT
-         \<le> SPEC
-            (\<lambda>x. (case x of
-                  (b, Ta, m', n') \<Rightarrow> do {
-                    ebrk \<leftarrow> RES UNIV;
-                    RETURN (ebrk, brkT, (if b then Ta else T), Ta, m', n')})
-                 \<le> SPEC
-                    (\<lambda>s'. (cdcl_twl_stgy_restart_prog_inv S o snd) s' \<and>
-                          (s', ebrkU, brkU, T, U, m, n)
-                          \<in> cdcl_algo_termination_early_rel))\<close>
-    (is \<open>_ \<le> SPEC (\<lambda>x. _ \<le> SPEC(\<lambda>s. ?I s \<and> _ \<in> ?term))\<close>)
+lemma  wf_cdcl_algo_termination_early_rel: \<open>wf cdcl_algo_termination_early_rel\<close> (is \<open>wf (?C \<union> ?D)\<close>)
 proof -
-  have [simp]: \<open>\<not>brkU\<close> \<open>\<not>ebrkU\<close>
-    using cond by auto
-  have struct_invs': \<open>cdcl_twl_restart W T' \<Longrightarrow> cdcl_twl_stgy\<^sup>*\<^sup>* T' V' \<Longrightarrow> twl_struct_invs V'\<close> for T' V'
-    using assms(3) cdcl_twl_restart_twl_struct_invs
-    by (metis (no_types, lifting) case_prodD rtranclp_cdcl_twl_stgy_twl_struct_invs)
-  have stgy_invs: \<open>cdcl_twl_restart W V' \<Longrightarrow> cdcl_twl_stgy\<^sup>*\<^sup>* V' W' \<Longrightarrow> twl_stgy_invs W'\<close> for V' W'
-    using assms(3) cdcl_twl_restart_twl_stgy_invs
-    by (metis (no_types, lifting) case_prodD cdcl_twl_restart_twl_struct_invs
-      rtranclp_cdcl_twl_stgy_twl_stgy_invs)
-  have res_no_clss_to_upd: \<open>cdcl_twl_restart U V \<Longrightarrow> clauses_to_update V = {#}\<close> for V
-    by (auto simp: cdcl_twl_restart.simps)
-  have res_no_confl: \<open>cdcl_twl_restart U V \<Longrightarrow> get_conflict V = None\<close> for V
-    by (auto simp: cdcl_twl_restart.simps)
-
-  have
-    struct_invs_S: \<open>twl_struct_invs S\<close> and
-    struct_invs_U: \<open>twl_struct_invs U\<close> and
-    twl_stgy_invs_U: \<open>twl_stgy_invs U\<close> and
-    \<open>brkU \<longrightarrow> final_twl_state U\<close> and
-    twl_res: \<open>cdcl_twl_stgy_restart_with_leftovers (S, 0, True) m T (U, n, True)\<close> and
-    clss_T: \<open>clauses_to_update U = {#}\<close> and
-    confl: \<open>\<not> brkU \<longrightarrow> get_conflict U = None\<close>
-    using inv unfolding cdcl_twl_stgy_restart_prog_inv_def prod.case comp_def snd_conv by fast+
-
-  have
-    cdcl_o: \<open>cdcl_twl_o\<^sup>*\<^sup>* V W\<close> and
-    conflict_W: \<open>get_conflict W \<noteq> None \<Longrightarrow> count_decided (get_trail W) = 0\<close> and
-    brk'_no_step: \<open>brkT \<Longrightarrow> final_twl_state W\<close> and
-    struct_invs_W: \<open>twl_struct_invs W\<close> and
-    stgy_invs_W: \<open>twl_stgy_invs W\<close> and
-    clss_to_upd_W: \<open>clauses_to_update W = {#}\<close> and
-    lits_to_upd_W: \<open>\<not> brkT \<longrightarrow> literals_to_update W \<noteq> {#}\<close> and
-    confl_W: \<open>\<not> brkT \<longrightarrow> get_conflict W = None\<close>
-    using other_inv unfolding final_twl_state_def by fast+
-
-  have \<open>cdcl_twl_stgy\<^sup>*\<^sup>* V W\<close>
-    by (meson cdcl_o assms(5) rtranclp_cdcl_twl_cp_stgyD rtranclp_cdcl_twl_o_stgyD
-        rtranclp_trans)
-  from twl_res have
-    STa: \<open>cdcl_twl_stgy_restart\<^sup>*\<^sup>* (S, 0, True) (T, n, True)\<close> and
-    TaT: \<open>cdcl_twl_stgy\<^sup>*\<^sup>* T U\<close> and
-    m: \<open>m = size (get_all_learned_clss T)\<close>
-    unfolding cdcl_twl_stgy_restart_with_leftovers_def prod.case snd_conv fst_conv
-    by blast+
-  have struct_invs_T: \<open>twl_struct_invs T\<close>
-    using STa rtranclp_cdcl_twl_stgy_restart_twl_struct_invs struct_invs_S by fastforce
-  have restart_prog_pre_W: \<open>restart_prog_pre W brkT\<close>
-    using confl_W stgy_invs_W struct_invs_W
-    unfolding restart_prog_pre_def
-    by fast
-
-  have UW: \<open>cdcl_twl_stgy\<^sup>*\<^sup>* U W\<close>
-    by (meson \<open>cdcl_twl_stgy\<^sup>*\<^sup>* V W\<close> local.cp rtranclp_cdcl_twl_cp_stgyD rtranclp_trans)
-    have TW: \<open>cdcl_twl_stgy\<^sup>*\<^sup>* T W\<close>
-      by (metis (no_types) TaT \<open>cdcl_twl_stgy\<^sup>*\<^sup>* V W\<close> local.cp
-        rtranclp_cdcl_twl_cp_stgyD rtranclp_tranclp_tranclp rtranclp_unfold)
-  have only_restart: \<open>?I (ebrk, False, if True then Y else T, Y, size (get_all_learned_clss Y), n)\<close> (is ?A) and
-     only_restart_term: \<open>((ebrk, False, (if True then Y else T), Y, size (get_all_learned_clss Y), n),
-        ebrkU, brkU, T, U, m, n)
-        \<in> ?term\<close> (is ?B)
-    if
-      \<open>True \<longrightarrow> f n < size (get_all_learned_clss W) - m\<close> and
-      m_size_W: \<open>True \<longrightarrow> m < size (get_all_learned_clss W)\<close> and
-      WY: \<open>cdcl_twl_restart_only W Y\<close> and
-      brkX and
-      X and
-      \<open>\<not> brkT\<close>
-    for X brkX Y ebrk
+  have A: \<open>{(T, S :: 'v twl_st_restart). twl_restart_inv S \<and> cdcl_twl_stgy_restart S T}\<^sup>+ =
+    {(T, S :: 'v twl_st_restart). twl_restart_inv S \<and> cdcl_twl_stgy_restart\<^sup>+\<^sup>+ S T}\<close> (is \<open>?A = ?B\<close>)
   proof -
-    have \<open>size (get_all_learned_clss T) \<le> size (get_all_learned_clss U)\<close>
-      using rtranclp_cdcl_twl_stgy_size_get_all_learned[of T U] TaT
-      by auto
-    have TW: \<open>cdcl_twl_stgy\<^sup>+\<^sup>+ T W\<close>
-      by (metis (no_types) TaT \<open>cdcl_twl_stgy\<^sup>*\<^sup>* V W\<close> lits_to_upd_W lits_to_update local.cp
-        rtranclp_cdcl_twl_cp_stgyD rtranclp_tranclp_tranclp rtranclp_unfold that(6))
-    have UW: \<open>cdcl_twl_stgy\<^sup>+\<^sup>+ U W\<close>
-      by (metis (mono_tags) Nitpick.rtranclp_unfold \<open>cdcl_twl_stgy\<^sup>*\<^sup>* V W\<close> lits_to_upd_W
-        lits_to_update local.cp that(6) tranclp_cdcl_twl_cp_stgyD tranclp_rtranclp_tranclp)
-    have \<open>twl_struct_invs Y\<close>
-      using WY cdcl_twl_restart_only_twl_struct_invs struct_invs_W by blast
-    moreover have \<open>twl_stgy_invs Y\<close>
-      using WY cdcl_twl_stgy_restart_only_twl_stgy_invs stgy_invs_W by blast
-    moreover have \<open>clauses_to_update Y = {#}\<close> \<open>get_conflict Y = None\<close>
-      using WY by (auto simp: cdcl_twl_restart_only.simps)
-    moreover {
-      have \<open>cdcl_twl_stgy_restart (T, n, True) (Y, n, True)\<close>
-        by (rule restart_noGC[OF _ _ WY])
-         (auto simp: m_size_W UW TW  m[symmetric])
-      then have \<open>cdcl_twl_stgy_restart_with_leftovers (S, 0, True)
-        (size (get_all_learned_clss Y)) Y (Y, n, True)\<close>
-        using STa
-        unfolding cdcl_twl_stgy_restart_with_leftovers_def
-        by auto
-    }
-    ultimately show ?A
-      using struct_invs_S
-      by (auto simp: cdcl_twl_stgy_restart_prog_inv_def)
-    have \<open>cdcl_twl_stgy_restart_with_leftovers1 (T, n, True) (Y, n, True)\<close>
-      using m_size_W
-      unfolding cdcl_twl_stgy_restart_with_leftovers1_def m
-      by (auto intro!: cdcl_twl_stgy_restart.intros(2)[of _ W] simp: WY TW UW)
-    then show ?B by (auto simp: struct_invs_T m)
-  qed
-  have full_restart: \<open>?I (ebrk, False, if True then Z else T, Z, size (get_all_learned_clss Z), n + 1)\<close> (is ?A)and
-    full_restart_term:
-      \<open>((ebrk, False, if True then Z else T, Z, size (get_all_learned_clss Z), n + 1), ebrkU, brkU, T, U, m, n)
-    \<in> ?term\<close> (is ?B)
-    if
-      \<open>restart_prog_pre W False\<close> and
-      m_size: \<open>True \<longrightarrow> f n < size (get_all_learned_clss W) - m\<close> and
-      \<open>True \<longrightarrow> m < size (get_all_learned_clss W)\<close> and
-      \<open>\<not> (brkX \<and> True \<and> \<not> False)\<close> and
-      WY: \<open>cdcl_twl_restart W Y\<close> and
-      X and
-      \<open>\<not> brkT\<close> and
-      YZ: \<open>cdcl_twl_stgy\<^sup>*\<^sup>* Y Z\<close> and
-      clss_Z: \<open>clauses_to_update Z = {#}\<close> and
-      confl_Z: \<open>get_conflict Z = None\<close>
-    for X brkX Y Z ebrk
-  proof -
-    have TW: \<open>cdcl_twl_stgy\<^sup>+\<^sup>+ T W\<close>
-      by (metis (no_types) TaT \<open>cdcl_twl_stgy\<^sup>*\<^sup>* V W\<close> lits_to_upd_W lits_to_update local.cp
-        rtranclp_cdcl_twl_cp_stgyD rtranclp_tranclp_tranclp rtranclp_unfold that(7))
-    have UW: \<open>cdcl_twl_stgy\<^sup>+\<^sup>+ U W\<close>
-      by (metis (mono_tags) Nitpick.rtranclp_unfold \<open>cdcl_twl_stgy\<^sup>*\<^sup>* V W\<close> lits_to_upd_W
-        lits_to_update local.cp that(7) tranclp_cdcl_twl_cp_stgyD tranclp_rtranclp_tranclp)
-    have UZ: \<open>cdcl_twl_stgy_restart (T, n, True) (Z, Suc n, True)\<close>
-      apply (rule restart_step[OF TW _ WY YZ])
-      using m_size
-      unfolding m[symmetric]
-      by (auto simp: m UW clss_Z confl_Z)
-    have \<open>twl_struct_invs Z\<close>
-      using struct_invs' WY YZ by blast
-    moreover have \<open>twl_stgy_invs Z\<close>
-      using WY YZ stgy_invs by blast
-    moreover have \<open>cdcl_twl_stgy_restart_with_leftovers (S, 0, True)
-        (size (get_all_learned_clss Z)) Z (Z, Suc n, True)\<close>
-        using STa UZ
-        by (auto simp: cdcl_twl_stgy_restart_with_leftovers_def)
-    ultimately show ?A
-      using struct_invs_S YZ WY clss_Z confl_Z
-      by (auto simp: cdcl_twl_stgy_restart_prog_inv_def)
-    have \<open>cdcl_twl_stgy_restart_with_leftovers1 (T, n, True) (Z, Suc n, True)\<close>
-      using UZ by (auto simp: cdcl_twl_stgy_restart_with_leftovers1_def)
-    then show ?B
-      by (auto simp: struct_invs_T)
-  qed
-  have no_restart: \<open>?I (ebrk, brkT, if False then W else T, W, m, n)\<close>
-    for ebrk :: bool
-    using struct_invs_S STa TW
-    by (auto simp: struct_invs_S struct_invs_W stgy_invs_W clss_to_upd_W confl_W
-      cdcl_twl_stgy_restart_with_leftovers_def m brk'_no_step cdcl_twl_stgy_restart_prog_inv_def)
-
-  have no_restart_term: \<open>cdcl_twl_stgy_restart_with_leftovers1 (U, n, True) (W, n, \<not> brkT)\<close>
-  proof -
-    have \<open>cdcl_twl_stgy\<^sup>+\<^sup>+ U W\<close> if \<open>\<not> cdcl_twl_stgy_restart (U, n, True) (W, n, \<not> brkT)\<close>
-    proof -
-      have "(\<not> brkT \<or> \<not> cdcl_twl_stgy\<^sup>*\<^sup>* U W) \<or> \<not> pcdcl_twl_final_state W"
-        using twl_restart_ops.cdcl_twl_stgy_restart.restart_full that by fastforce
-      then show "cdcl_twl_stgy\<^sup>+\<^sup>+ U W"
-        by (metis (no_types) Nitpick.rtranclp_unfold \<open>cdcl_twl_stgy\<^sup>*\<^sup>* V W\<close> brk'_no_step
-          final_twl_state_def lits_to_upd_W lits_to_update local.cp pcdcl_twl_final_state_def
-          rtranclp_cdcl_twl_cp_stgyD tranclp_rtranclp_tranclp)
-    qed
-    moreover have False if \<open>\<not>cdcl_twl_stgy_restart (U, n, True) (W, n, False)\<close> and brkT
-      using UW brk'_no_step final_twl_state_def pcdcl_twl_final_state_def that
-        twl_restart_ops.cdcl_twl_stgy_restart.restart_full by blast
+    have \<open>(x, y) \<in> ?A \<Longrightarrow> (x, y) \<in> ?B\<close> for x y
+      by (induction rule: trancl_induct)
+        auto
+    moreover have \<open>cdcl_twl_stgy_restart\<^sup>+\<^sup>+ S T \<Longrightarrow> twl_restart_inv S \<Longrightarrow> (T, S) \<in> ?A\<close> for S T
+      apply (induction rule: tranclp_induct)
+      subgoal by auto
+      subgoal for T U
+        by (rule trancl_into_trancl2[of _ T])
+          (use rtranclp_cdcl_twl_stgy_restart_twl_restart_inv[of S T] in \<open>simp_all add: tranclp_into_rtranclp\<close>)
+      done
     ultimately show ?thesis
-      by (auto simp: cdcl_twl_stgy_restart_with_leftovers1_def)
+      by blast
   qed
-  have \<open>cdcl_twl_stgy\<^sup>+\<^sup>+ U W \<or> U = W\<close>
-    by (meson UW rtranclp_unfold)
-  then have no_restart_term: \<open>((ebrk, brkT, if False then W else T, W, m, n), ebrkU, brkU, T, U, m, n)
-    \<in> ?term\<close> for ebrk
-    using no_restart_term
-    apply (auto simp: struct_invs_T struct_invs_U)
-    by (metis (no_types, lifting) \<open>cdcl_twl_stgy\<^sup>*\<^sup>* V W\<close> lits_to_upd_W lits_to_update local.cp
-      rtranclp_cdcl_twl_cp_stgyD rtranclp_into_tranclp1 rtranclp_unfold tranclp_idemp)+
-
-  show ?thesis
-    unfolding restart_prog_def restart_required_def
-    apply (refine_vcg; remove_dummy_vars)
-    subgoal by (rule restart_prog_pre_W)
-    subgoal for X brkX Y
-      by (rule only_restart)
-    subgoal for X brkX Y
-      by (rule only_restart_term)
-    subgoal for X brkX Y Z
-      by (rule full_restart)
-    subgoal for X brkX Y Z
-      by (rule full_restart_term)
-    subgoal for brk brk'
-      by (rule no_restart)
-    subgoal for brk brk'
-      by (rule no_restart_term)
-    done
+  have \<open>wf ?D\<close>
+    by (rule wf_no_loop) auto
+  moreover have \<open>wf ?C\<close>
+    by (rule wf_if_measure_in_wf[OF wf_trancl[OF wf_cdcl_twl_stgy_restart, unfolded A],
+        of _  \<open>\<lambda>(_, brkT, R, S, T, n, n'). (R, S, T, n, n', \<not>brkT)\<close>])
+      auto
+  moreover have \<open>?D O ?C \<subseteq> ?D\<close>
+    by auto
+  ultimately show ?thesis
+    apply (subst Un_commute)
+    by (rule wf_union_compatible)
 qed
 
 definition cdcl_twl_stgy_restart_prog_bounded :: "'v twl_st \<Rightarrow> (bool \<times> 'v twl_st) nres" where
@@ -356,17 +167,181 @@ definition cdcl_twl_stgy_restart_prog_bounded :: "'v twl_st \<Rightarrow> (bool 
     ebrk \<leftarrow> RES UNIV;
     (ebrk, _, _, T, _, n) \<leftarrow> WHILE\<^sub>T\<^bsup>cdcl_twl_stgy_restart_prog_inv S\<^sub>0 o snd\<^esup>
       (\<lambda>(ebrk, brk, _). \<not>brk \<and> \<not>ebrk)
-      (\<lambda>(ebrk, brk, S', S, m, n).
+      (\<lambda>(ebrk, brk, Q, R, S, m, n).
       do {
         T \<leftarrow> unit_propagation_outer_loop S;
         (brk, T) \<leftarrow> cdcl_twl_o_prog T;
-        (b, T, m, n) \<leftarrow> restart_prog T m n brk;
+        (Q, R, T, m, n) \<leftarrow> restart_prog Q R T m n brk;
 	ebrk \<leftarrow> RES UNIV;
-        RETURN (ebrk, brk, if b then T else S', T, m, n)
+        RETURN (ebrk, brk, Q, R, T, m, n)
       })
-      (ebrk, False, S\<^sub>0, S\<^sub>0, size (get_all_learned_clss S\<^sub>0), 0);
+      (ebrk, False, S\<^sub>0, S\<^sub>0, S\<^sub>0, 0, 0);
     RETURN (ebrk, T)
   }\<close>
+
+
+lemma cdcl_twl_stgy_prog_bounded_spec:
+  assumes
+    \<open>iebrk \<in> UNIV\<close> and
+    inv: \<open>(cdcl_twl_stgy_restart_prog_inv S \<circ> snd) (ebrk, brk, S, T, U, m, n)\<close> and
+    cond: \<open>case (ebrk, brk, S, T, U, m, n) of
+     (ebrk, brk, uu_) \<Rightarrow> \<not> brk \<and> \<not> ebrk\<close> and
+    other_inv: \<open>cdcl_twl_o_prog_spec V (brkW, W)\<close> and
+    \<open>twl_struct_invs V\<close> and
+    \<open>cdcl_twl_cp\<^sup>*\<^sup>* U V\<close> and
+    \<open>literals_to_update V = {#}\<close> and
+    \<open>\<forall>S'. \<not> cdcl_twl_cp V S'\<close> and
+    \<open>twl_stgy_invs V\<close>
+  shows \<open>restart_prog S T W m n brkW
+         \<le> SPEC
+            (\<lambda>x. (case x of (Q, R, T, m, n) \<Rightarrow> do {
+                                ebrk \<leftarrow> RES UNIV;
+                                RETURN (ebrk, brkW, Q, R, T, m, n)
+                              })
+                 \<le> SPEC
+                    (\<lambda>s'. (cdcl_twl_stgy_restart_prog_inv S \<circ> snd) s' \<and>
+                          (s', ebrk, brk, S, T, U, m, n)
+                          \<in> cdcl_algo_termination_early_rel))\<close>
+    (is \<open>_ \<le> SPEC (\<lambda>x. _ \<le> SPEC(\<lambda>s. ?I s \<and> _ \<in> ?term))\<close>)
+proof -
+
+  have [simp]: \<open>\<not>brk\<close> \<open>\<not>ebrk\<close>
+    using cond by auto
+  have struct_invs': \<open>cdcl_twl_restart W T' \<Longrightarrow> cdcl_twl_stgy\<^sup>*\<^sup>* T' V' \<Longrightarrow> twl_struct_invs V'\<close> for T' V'
+    using assms(3) cdcl_twl_restart_twl_struct_invs
+      by (metis (no_types, lifting) assms(4) case_prodD rtranclp_cdcl_twl_stgy_twl_struct_invs)
+  have stgy_invs: \<open>cdcl_twl_restart W V' \<Longrightarrow> cdcl_twl_stgy\<^sup>*\<^sup>* V' W' \<Longrightarrow> twl_stgy_invs W'\<close> for V' W'
+    using assms(3) cdcl_twl_restart_twl_stgy_invs
+    by (metis (no_types, lifting) assms(4) case_prodD cdcl_twl_restart_twl_struct_invs
+      rtranclp_cdcl_twl_stgy_twl_stgy_invs)
+
+  have res_no_clss_to_upd: \<open>cdcl_twl_restart U V \<Longrightarrow> clauses_to_update V = {#}\<close> for V
+    by (auto simp: cdcl_twl_restart.simps)
+  have res_no_confl: \<open>cdcl_twl_restart U V \<Longrightarrow> get_conflict V = None\<close> for V
+    by (auto simp: cdcl_twl_restart.simps)
+
+  have
+    struct_invs_S: \<open>twl_struct_invs S\<close> and
+    struct_invs_T: \<open>twl_struct_invs T\<close> and
+    struct_invs_U: \<open>twl_struct_invs U\<close> and
+    twl_stgy_invs_S: \<open>twl_stgy_invs S\<close> and
+    twl_stgy_invs_T: \<open>twl_stgy_invs T\<close> and
+    twl_stgy_invs_U: \<open>twl_stgy_invs U\<close> and
+    \<open>brk \<longrightarrow> final_twl_state U\<close> and
+    twl_res: \<open>cdcl_twl_stgy_restart\<^sup>*\<^sup>* (S, S, S, 0, 0, True) (S, T, U, m, n, \<not> brk)\<close> and
+    clss_T: \<open>clauses_to_update U = {#}\<close> and
+    confl: \<open>\<not> brk \<longrightarrow> get_conflict U = None\<close> and
+    STU_inv: \<open>pcdcl_stgy_restart_inv (pstate\<^sub>W_of S, pstate\<^sub>W_of T, pstate\<^sub>W_of U, m, n, \<not> brk)\<close>
+    using inv unfolding cdcl_twl_stgy_restart_prog_inv_alt_def prod.case comp_def snd_conv
+      twl_restart_inv_def twl_stgy_restart_inv_def by fast+
+
+  have
+    cdcl_o: \<open>cdcl_twl_o\<^sup>*\<^sup>* V W\<close> and
+    conflict_W: \<open>get_conflict W \<noteq> None \<Longrightarrow> count_decided (get_trail W) = 0\<close> and
+    brk'_no_step: \<open>brkW \<Longrightarrow> final_twl_state W\<close> and
+    struct_invs_W: \<open>twl_struct_invs W\<close> and
+    stgy_invs_W: \<open>twl_stgy_invs W\<close> and
+    clss_to_upd_W: \<open>clauses_to_update W = {#}\<close> and
+    lits_to_upd_W: \<open>\<not> brkW \<longrightarrow> literals_to_update W \<noteq> {#}\<close> and
+    confl_W: \<open>\<not> brkW \<longrightarrow> get_conflict W = None\<close>
+    using other_inv unfolding final_twl_state_def by fast+
+
+  have \<open>cdcl_twl_stgy\<^sup>*\<^sup>* V W\<close>
+    by (meson cdcl_o assms(5) rtranclp_cdcl_twl_cp_stgyD rtranclp_cdcl_twl_o_stgyD
+      rtranclp_trans)
+
+  have restart_W: \<open>restart_prog_pre W brkW\<close>
+    using struct_invs_W stgy_invs_W confl_W unfolding restart_prog_pre_def by auto
+  have [simp]: \<open>twl_restart_inv (S, S, S, 0, 0, True)\<close> \<open>twl_stgy_restart_inv (S, S, S, 0, 0, True)\<close>
+    using struct_invs_S twl_stgy_invs_S
+    by (auto simp: twl_restart_inv_def twl_stgy_restart_inv_def pcdcl_stgy_restart_inv_def
+      twl_struct_invs_def)
+  have UW: \<open>cdcl_twl_stgy_restart\<^sup>*\<^sup>* (S, T, U, m, n, True) (S, T, W, m, n, True)\<close>
+    apply (rule cdcl_twl_stgy_restart_rtranclpI)
+    by (meson \<open>cdcl_twl_stgy\<^sup>*\<^sup>* V W\<close> assms(6) rtranclp_cdcl_twl_cp_stgyD rtranclp_trans)
+  have restart_only: \<open>?I (ebrk', False, S, X, X, Suc m, n)\<close> (is ?A) and
+    restart_only_term: \<open>((ebrk', False, S, X, X, Suc m, n), ebrk, brk, S, T, U, m, n) \<in> ?term\<close> (is ?B)
+    if 
+      \<open>restart_prog_pre W False\<close> and
+      less: \<open>True \<longrightarrow>
+      size (get_all_learned_clss T) < size (get_all_learned_clss W)\<close> and
+      WX: \<open>cdcl_twl_restart_only W X\<close> and
+      \<open>ebrk' \<in> UNIV\<close> and
+      y and
+      x
+     for x y X ebrk'
+  proof -
+    have WX': \<open>cdcl_twl_stgy_restart (S, T, W, m, n, True) (S, X, X, Suc m, n, True)\<close>
+      by (rule cdcl_twl_stgy_restart.intros)
+        (use less WX in auto)
+    show ?A
+      using UW WX twl_res WX' clss_to_upd_W
+      by (auto simp: cdcl_twl_stgy_restart_prog_inv_def cdcl_twl_restart_only.simps)
+    show ?B
+      using STU_inv UW WX'
+      by (auto simp: twl_restart_inv_def struct_invs_S struct_invs_T struct_invs_U)
+  qed
+  have GC: \<open>?I (ebrk', False, Y, Y, Y, m, Suc n)\<close> (is ?A) and
+    GC_term: \<open>((ebrk', False, Y, Y, Y, m, Suc n), ebrk, brk, S, T, U, m, n) \<in> ?term\<close> (is ?B)
+    if 
+      \<open>restart_prog_pre W False\<close> and
+      less: \<open>True \<longrightarrow> f n < size (get_all_learned_clss W) - size (get_all_learned_clss S)\<close> and
+      WX: \<open>cdcl_twl_restart W X\<close> and
+      \<open>ebrk' \<in> UNIV\<close> and
+      x and
+      \<open>\<not> brkW\<close> and
+      XY: \<open>cdcl_twl_stgy\<^sup>*\<^sup>* X Y\<close>
+        \<open>clauses_to_update Y = {#}\<close>
+        \<open>get_conflict Y = None\<close>
+    for x X Y ebrk'
+  proof -
+    have WX': \<open>cdcl_twl_stgy_restart (S, T, W, m, n, True) (Y, Y, Y, m, Suc n, True)\<close>
+      by (rule cdcl_twl_stgy_restart.intros)
+        (use less WX XY in auto)
+    show ?A
+      using UW WX twl_res WX' XY
+      by (auto simp: cdcl_twl_stgy_restart_prog_inv_def)
+    show ?B
+      using STU_inv UW WX'
+      by (auto simp: twl_restart_inv_def struct_invs_S struct_invs_T struct_invs_U)
+  qed
+  have continue: \<open>?I (ebrk', brkW, S, T, W, m, n)\<close> (is ?A) and
+    continue_term: \<open>((ebrk', brkW, S, T, W, m, n), ebrk, brk, S, T, U, m, n) \<in> ?term\<close> (is ?B) for ebrk'
+  proof -
+    show ?A
+      using brk'_no_step confl_W clss_to_upd_W UW twl_res
+        cdcl_twl_stgy_restart.intros(4)[of W S T m n]
+      apply (cases brkW)
+      apply (auto simp add: cdcl_twl_stgy_restart_prog_inv_def)
+      apply (metis (no_types, lifting) final_twl_state_def pcdcl_twl_final_state_def rtranclp.simps rtranclp_trans)
+      done
+    have\<open>cdcl_twl_stgy\<^sup>+\<^sup>+ V W\<close> if \<open>\<not>brkW\<close>
+      using  \<open>cdcl_twl_stgy\<^sup>*\<^sup>* V W\<close> lits_to_upd_W that assms(7) unfolding rtranclp_unfold
+      by auto
+    then have [simp]: \<open>cdcl_twl_stgy_restart\<^sup>+\<^sup>+ (S, T, U, m, n, True) (S, T, W, m, n, True)\<close> if \<open>\<not>brkW\<close>
+      by (meson assms(6) cdcl_twl_stgy_restart_tranclpI
+        rtranclp_cdcl_twl_cp_stgyD rtranclp_tranclp_tranclp that)
+
+    show ?B
+      using STU_inv brk'_no_step
+      apply (cases brkW)
+      by (auto simp: twl_restart_inv_def struct_invs_S struct_invs_T struct_invs_U)
+  qed
+  show ?thesis 
+    unfolding restart_prog_def restart_required_def GC_required_def
+    apply (refine_vcg; remove_dummy_vars)
+    subgoal by (rule restart_W)
+    subgoal by (rule restart_only)
+    subgoal by (rule restart_only_term)
+    subgoal by (rule GC)
+    subgoal by (rule GC_term)
+    subgoal
+      by (rule continue)
+    subgoal
+      by (rule continue_term)
+    done
+qed
+
 
 lemma (in twl_restart) cdcl_twl_stgy_prog_bounded_spec:
   assumes \<open>twl_struct_invs S\<close> and \<open>twl_stgy_invs S\<close> and \<open>clauses_to_update S = {#}\<close> and
@@ -383,35 +358,6 @@ proof -
         WHILEIT_rule[where
            R = \<open>cdcl_algo_termination_early_rel\<close>];
         remove_dummy_vars)
-    subgoal
-      by (rule wf_cdcl_algo_termination_early_rel)
-    subgoal using assms
-      by (auto simp: cdcl_twl_stgy_restart_prog_inv_def cdcl_twl_stgy_restart_with_leftovers_def)
-    subgoal using assms
-      by (auto dest: rtranclp_cdcl_twl_stgy_restart_twl_struct_invs
-        simp: cdcl_twl_stgy_restart_prog_inv_def cdcl_twl_stgy_restart_with_leftovers_def)
-    subgoal using assms
-      by (auto simp: cdcl_twl_stgy_restart_prog_inv_def cdcl_twl_stgy_restart_with_leftovers_def
-        dest!: rtranclp_cdcl_twl_stgy_restart_clauses_to_update)
-    subgoal using assms
-      by (auto simp: cdcl_twl_stgy_restart_prog_inv_def cdcl_twl_stgy_restart_with_leftovers_def
-        dest!: rtranclp_cdcl_twl_stgy_restart_get_conflict)
-    subgoal
-      using assms
-      by (auto simp: cdcl_twl_stgy_restart_prog_inv_def cdcl_twl_stgy_restart_with_leftovers_def
-        dest: rtranclp_cdcl_twl_stgy_restart_twl_stgy_invs)
-    subgoal
-      using assms
-      by (auto simp: cdcl_twl_stgy_restart_prog_inv_def cdcl_twl_stgy_restart_with_leftovers_def
-        no_step_cdcl_twl_cp_no_step_cdcl\<^sub>W_cp)
-    subgoal by fast
-    subgoal for brkU U T m n V brkT W
-      by (rule restart_prog_spec)
-    subgoal for init_ebrk brkT T' m n ebrk T
-      by (rule_tac x=T' in exI) (auto simp: cdcl_twl_stgy_restart_prog_inv_def)
-    done
-qed
-
 
 lemma cdcl_twl_stgy_restart_prog_spec:
   fixes S :: \<open>'v twl_st\<close>
